src/FrameStack/SubstSemanticsLabeledLemmas.v
@@ -8,7 +8,7 @@ From CoreErlang.FrameStack Require Export
 From stdpp Require Export list option.
 Import ListNotations.
 
-Corollary side_effect_ac_value : forall fs r fs' r' l0,
+Lemma side_effect_ac_value : forall fs r fs' r' l0,
   ⟨ fs, r ⟩ -⌊ Some ((AtomCreation, l0):SideEffect) ⌋->ₗ ⟨ fs', r' ⟩ ->
   exists av, l0 = [VLit (Atom av)].
 Proof.
@@ -94,9 +94,9 @@ Proof.
       destruct (params =? (length (vl ++ [v])))%nat; try discriminate.
 Qed.
 
-Corollary transitive_eval :
-  forall {n e e' l fs fs'}, ⟨ fs, e ⟩ -[ n, l ]->ₗ ⟨ fs', e' ⟩ ->
-  forall {n' e'' l' fs''},  ⟨ fs', e' ⟩ -[ n', l' ]->ₗ ⟨ fs'', e'' ⟩
+Theorem transitive_eval_labeled :
+  forall {n e e'} l {fs fs'}, ⟨ fs, e ⟩ -[ n, l ]->ₗ ⟨ fs', e' ⟩ ->
+  forall {n' e''} l' {fs''},  ⟨ fs', e' ⟩ -[ n', l' ]->ₗ ⟨ fs'', e'' ⟩
 ->
   ⟨ fs, e ⟩ -[ n + n', l ++ l' ]->ₗ ⟨ fs'', e'' ⟩.
 Proof.
@@ -106,17 +106,17 @@ Proof.
   destruct s; rewrite H0; auto.
 Qed.
 
-Corollary transitive_any_eval :
-  forall {e e' l fs fs'}, ⟨ fs, e ⟩ -[ l ]->ₗ* ⟨ fs', e' ⟩ ->
-  forall {e'' l' fs''},  ⟨ fs', e' ⟩ -[ l' ]->ₗ* ⟨ fs'', e'' ⟩
+Corollary transitive_any_eval_labeled :
+  forall {e e'} l {fs fs'}, ⟨ fs, e ⟩ -[ l ]->ₗ* ⟨ fs', e' ⟩ ->
+  forall {e''} l' {fs''},  ⟨ fs', e' ⟩ -[ l' ]->ₗ* ⟨ fs'', e'' ⟩
 ->
   ⟨ fs, e ⟩ -[ l ++ l' ]->ₗ* ⟨ fs'', e'' ⟩.
 Proof.
-  intros. destruct H, H0. pose proof (transitive_eval H H0).
+  intros. destruct H, H0. pose proof (transitive_eval_labeled _ H _ H0).
   unfold step_any_non_terminal. eexists. exact H1.
 Qed.
 
-Corollary step_determinism {e e' l fs fs'} :
+Theorem step_determinism_labeled {e e' l fs fs'} :
   ⟨ fs, e ⟩ -⌊ l ⌋->ₗ ⟨ fs', e' ⟩ ->
   (forall {l' fs'' e''}, ⟨ fs, e ⟩ -⌊ l' ⌋->ₗ ⟨ fs'', e'' ⟩
   -> l = l' /\ fs'' = fs' /\ e'' = e').
@@ -126,14 +126,14 @@ Proof.
   - rewrite <- H0 in H8. now inv H8.
 Qed.
 
-Corollary value_nostep v :
+Lemma value_nostep_labeled v :
   is_result v ->
   forall fs' v' l, ⟨[], v⟩ -⌊l⌋->ₗ ⟨fs' , v'⟩ -> False.
 Proof.
   intros H fs' v' l' HD. inversion H; subst; inversion HD.
 Qed.
 
-Corollary step_rt_determinism {r r' fs fs' l k} :
+Theorem step_rt_determinism_labeled {r r' fs fs' l k} :
   ⟨fs, r⟩ -[k, l]->ₗ ⟨fs', r'⟩
 ->
   (forall {fs'' r'' l''}, ⟨fs, r⟩ -[k, l'']->ₗ ⟨fs'', r''⟩ -> l = l'' /\ fs' = fs'' /\ r' = r'').
@@ -141,12 +141,12 @@ Proof.
   intro. induction H; intros.
   * inv H. firstorder.
   * inv H2.
-    pose proof (step_determinism H H4) as [? [? ?]]. subst.
+    pose proof (step_determinism_labeled H H4) as [? [? ?]]. subst.
     specialize (IHstep_rt _ _ _ H5) as [? [? ?]]. subst.
     firstorder.
 Qed.
 
-Corollary create_result_closed :
+Lemma create_result_closed :
   forall vl ident r eff,
     Forall (fun v => VALCLOSED v) vl ->
     ICLOSED ident ->
@@ -194,7 +194,7 @@ Proof.
     - unfold badarity. constructor. constructor. auto.
 Qed.
 
-Corollary step_closedness : forall F e F' e' l,
+Theorem step_closedness_labeled : forall F e F' e' l,
    ⟨ F, e ⟩ -⌊l⌋->ₗ ⟨ F', e' ⟩ -> FSCLOSED F -> REDCLOSED e
 ->
   FSCLOSED F' /\ REDCLOSED e'.
@@ -266,12 +266,12 @@ Proof.
   * rewrite Nat.add_0_r in *. do 2 (constructor; auto).
 Qed.
 
-Corollary step_any_closedness : forall Fs Fs' e v k l,
+Theorem step_any_closedness_labeled : forall Fs Fs' e v k l,
    ⟨ Fs, e ⟩ -[k , l]->ₗ ⟨Fs', v⟩ -> FSCLOSED Fs -> REDCLOSED e
 ->
   REDCLOSED v /\ FSCLOSED Fs'.
 Proof.
-  intros. induction H; auto. apply step_closedness in H. destruct H.
+  intros. induction H; auto. apply step_closedness_labeled in H. destruct H.
   apply (IHstep_rt ). all: auto.
 Qed.
 
@@ -280,11 +280,11 @@ Corollary step_any_non_terminal_closedness : forall F e l F' e',
 -> REDCLOSED e' /\ FSCLOSED F'.
 Proof.
   intros F e l F' e' H. induction H; intros. destruct H. auto.
-  apply step_closedness in H. inv H.
-  apply (step_any_closedness _ _ _ _ _ _ H2 H4 H5). all: assumption.
+  apply step_closedness_labeled in H. inv H.
+  apply (step_any_closedness_labeled _ _ _ _ _ _ H2 H4 H5). all: assumption.
 Qed.
 
-Corollary transitive_eval_rev : forall Fs Fs' e e' k1 l1,
+Lemma transitive_eval_rev_labeled : forall Fs Fs' e e' k1 l1,
   ⟨ Fs, e ⟩ -[k1 , l1]->ₗ ⟨ Fs', e' ⟩->
   forall Fs'' e'' k2 l2,
   ⟨ Fs, e ⟩ -[k1 + k2 , l1 ++ l2]->ₗ ⟨ Fs'', e'' ⟩
@@ -297,21 +297,21 @@ Proof.
     destruct s; subst.
     + inv H2. destruct s0.
       * inv H7. eapply IHstep_rt.
-        destruct (step_determinism H H3).
+        destruct (step_determinism_labeled H H3).
         destruct H2. subst. assumption.
       * inv H7.
-        destruct (step_determinism H H3).
+        destruct (step_determinism_labeled H H3).
         inv H2.
     + inv H2. destruct s.
       * inv H7.
-        destruct (step_determinism H H3).
+        destruct (step_determinism_labeled H H3).
         inv H1.
       * inv H7. eapply IHstep_rt.
-        destruct (step_determinism H H3).
+        destruct (step_determinism_labeled H H3).
         destruct H2. subst. assumption.
 Qed.
 
-Corollary frame_indep_step : forall e F F' Fs e' l,
+Lemma frame_indep_step_labeled : forall e F F' Fs e' l,
   ⟨ F :: Fs, e ⟩ -⌊l⌋->ₗ ⟨ F' :: Fs, e' ⟩
 ->
   forall Fs', ⟨ F :: Fs', e ⟩ -⌊l⌋->ₗ ⟨ F' :: Fs', e' ⟩.
@@ -325,7 +325,7 @@ Proof.
   all: try (apply cons_neq in H5; contradiction).
 Qed.
 
-Corollary frame_indep_red : forall e F Fs e' l,
+Lemma frame_indep_red_labeled : forall e F Fs e' l,
   ⟨ F :: Fs, e ⟩ -⌊l⌋->ₗ ⟨ Fs, e' ⟩
 ->
   forall Fs', ⟨ F :: Fs', e ⟩ -⌊l⌋->ₗ ⟨ Fs', e' ⟩.
@@ -337,7 +337,7 @@ Proof.
   all: put (@length Frame : FrameStack -> nat) on H3 as H3L; simpl in H3L; lia.
 Qed.
 
-Corollary frame_indep_core : forall k e Fs Fs' v l,
+Theorem frame_indep_core_labeled : forall k e Fs Fs' v l,
   ⟨ Fs, e ⟩ -[k , l]->ₗ ⟨ Fs', v ⟩
 ->
   forall Fs'', ⟨ Fs ++ Fs'', e ⟩ -[k , l]->ₗ ⟨ Fs' ++ Fs'', v ⟩.
@@ -353,15 +353,15 @@ Proof.
     all: try apply H2; auto.
 Qed.
 
-Corollary frame_indep_nil : forall k e Fs v l,
+Corollary frame_indep_nil_labeled : forall k e Fs v l,
   ⟨ Fs, e ⟩ -[k , l]->ₗ ⟨ [], v ⟩
 ->
   forall Fs', ⟨ Fs ++ Fs', e ⟩ -[k , l]->ₗ ⟨ Fs', v ⟩.
 Proof.
-  intros. eapply frame_indep_core in H. exact H.
+  intros. eapply frame_indep_core_labeled in H. exact H.
 Qed.
 
-Corollary params_eval :
+Lemma params_eval_labeled :
   forall vals ident vl exps e Fs (v : Val),
   ⟨ FParams ident vl ((map VVal vals) ++ e :: exps) :: Fs, RValSeq [v]⟩ -[1 + 2 * length vals , []]->ₗ
   ⟨ FParams ident (vl ++ v :: vals) exps :: Fs, e⟩.
@@ -377,7 +377,7 @@ Proof.
     all: simpl; auto.
 Qed.
 
-Corollary params_eval_create :
+Lemma params_eval_create :
   forall vals ident vl Fs (v : Val) r eff',
   Some (r, eff') = create_result ident (vl ++ v :: vals) ->
   ⟨ FParams ident vl (map VVal vals) :: Fs, RValSeq [v]⟩ -[1 + 2 * length vals, match eff' with
@@ -398,7 +398,7 @@ Proof.
     reflexivity. reflexivity.
 Qed.
 
-Corollary terminates_in_k_step :
+Lemma terminates_in_k_step :
   forall fs e fs' e' k sl l, ⟨ fs, e ⟩ -⌊ l ⌋->ₗ ⟨ fs', e' ⟩ ->
   | fs', e' | sl – k ↓ ->
   | fs, e | (option_cons l sl) – S k ↓.
@@ -407,8 +407,8 @@ Proof.
   all: econstructor; eassumption.
 Qed.
 
-Corollary semantic_iff_termination :
-  forall k e fs l, terminates_in_k_l_sem fs e k l <-> | fs, e | l – k ↓.
+Theorem semantic_iff_termination :
+  forall k e fs l, terminates_in_k_sem_labeled fs e k l <-> | fs, e | l – k ↓.
 Proof.
   split.
   {
@@ -417,10 +417,10 @@ Proof.
       inversion HD; subst. now constructor.
     * destruct H as [res [Hres HD]].
       inversion HD; subst.
-      assert (terminates_in_k_l_sem fs' e' k l0). {
+      assert (terminates_in_k_sem_labeled fs' e' k l0). {
         eexists. split; eassumption.
       }
-      unfold terminates_in_k_l_sem in H.
+      unfold terminates_in_k_sem_labeled in H.
       apply IHk in H.
       eapply terminates_in_k_step.
       apply H0. apply H.
@@ -465,7 +465,7 @@ Definition option_tail {A} (l : option A) (sl : list A)
   | None => sl
   end.
 
-Corollary terminates_step :
+Lemma terminates_step :
   forall n fs e l, | fs, e | l – n ↓ -> forall fs' e' l', ⟨fs, e⟩ -⌊l'⌋->ₗ ⟨fs', e'⟩
 ->
   | fs', e' | (option_tail l' l) – n - 1↓.
@@ -475,7 +475,7 @@ Proof.
     - subst. inversion H1; subst. inversion H0.
     - subst. inversion H1; subst. inversion H0.
   * destruct H.
-    inv H1. apply (step_determinism H0) in H3.
+    inv H1. apply (step_determinism_labeled H0) in H3.
     inv H3. inv H2.
     assert (exists y, is_result y /\ ⟨ fs', e' ⟩ -[ n , l0 ]->ₗ ⟨ [], y ⟩). { 
       eexists. eauto. }
@@ -483,7 +483,7 @@ Proof.
     destruct s; simpl; rewrite Nat.sub_0_r; assumption.
 Qed.
 
-Corollary term_step_term_no_skip :
+Lemma term_step_term_no_skip :
   forall k n fs e l1 l2, | fs, e | l1 ++ l2 – n ↓ 
   -> forall fs' e' , ⟨fs, e⟩ -[k , l1]->ₗ ⟨fs', e'⟩
 ->
@@ -500,7 +500,7 @@ Proof.
       eapply IHk in H3. exact H3. exact H2.
 Qed.
 
-Corollary term_step_term :
+Lemma term_step_term_labeled :
   forall k n fs e l l1, | fs, e | l – n ↓ 
   -> forall fs' e' , ⟨fs, e⟩ -[k , l1]->ₗ ⟨fs', e'⟩
 ->
@@ -519,7 +519,7 @@ Proof.
       eapply IHk in H3. exact H3. exact H2.
 Qed.
 
-Corollary step_term_term :
+Lemma step_term_term_labeled :
   forall k n fs e fs' e' l1 l2,
   ⟨fs, e⟩ -[k , l1]->ₗ ⟨fs', e'⟩ -> | fs', e' | l2 – n - k ↓ -> n >= k 
 ->
@@ -527,11 +527,11 @@ Corollary step_term_term :
 Proof.
   intros. apply semantic_iff_termination.
   apply semantic_iff_termination in H0. destruct H0, H0.
-  pose proof (transitive_eval H H2). replace (k+(n-k)) with n in H3 by lia.
+  pose proof (transitive_eval_labeled _ H _ H2). replace (k+(n-k)) with n in H3 by lia.
   eexists. eauto.
 Qed.
 
-Corollary step_term_term_plus :
+Lemma step_term_term_plus_labeled :
   forall k k2 fs e fs' e' l1 l2, 
   ⟨fs, e⟩ -[k , l1]->ₗ ⟨fs', e'⟩ -> | fs', e' | l2 – k2 ↓
 ->
@@ -539,7 +539,7 @@ Corollary step_term_term_plus :
 Proof.
   intros. apply semantic_iff_termination.
   apply semantic_iff_termination in H0. destruct H0, H0.
-  pose proof (transitive_eval H H1).
+  pose proof (transitive_eval_labeled _ H _ H1).
   eexists. eauto.
 Qed.
 
@@ -597,7 +597,7 @@ Proof.
     - left. constructor.
 Qed.
 
-Corollary Private_params_exp_eval :
+Lemma Private_params_exp_eval :
   forall exps ident vl Fs (e : Exp) n (l : SideEffectList),
   | FParams ident vl exps :: Fs, e | l – n ↓ ->
   (forall m : nat,
@@ -613,14 +613,14 @@ Proof.
   induction exps; intros.
   * apply H0 in H as H'. 2: lia.
     destruct H' as [res [k [ll [Hres [Hd Hlt]]]]].
-    eapply frame_indep_nil in Hd.
+    eapply frame_indep_nil_labeled in Hd.
 (*    specialize (H1 _ _ _ _ _ Hd).
     eapply H1 in H. *)
-    eapply term_step_term in H. 2: exact Hd. simpl in *.
+    eapply term_step_term_labeled in H. 2: exact Hd. simpl in *.
     inv Hres.
     - do 3 eexists. split. 2: split.
       2: {
-        eapply transitive_eval. exact Hd.
+        eapply transitive_eval_labeled. exact Hd.
         eapply step_trans. constructor. reflexivity. apply step_refl.
         reflexivity.
       }
@@ -630,7 +630,7 @@ Proof.
       inv H. destruct (create_result_is_not_box ident (vl ++ [v]) res l0); auto.
       + do 3 eexists. split. 2: split.
         2: {
-          eapply transitive_eval. exact Hd.
+          eapply transitive_eval_labeled. exact Hd.
           eapply step_trans. econstructor. eassumption. apply step_refl.
           reflexivity.
         }
@@ -639,11 +639,11 @@ Proof.
       (* if create_result was a function application: *)
       + inv H. apply H0 in H8 as H8'.
         destruct H8' as [res2 [k2 [l2 [Hres2 [Hd2 Hlt2]]]]]. 2: lia.
-        eapply frame_indep_nil in Hd2.
-        eapply term_step_term in H8. 2: exact Hd2.
+        eapply frame_indep_nil_labeled in Hd2.
+        eapply term_step_term_labeled in H8. 2: exact Hd2.
         do 3 eexists. split. 2: split.
         2: {
-          eapply transitive_eval. exact Hd.
+          eapply transitive_eval_labeled. exact Hd.
           eapply step_trans. econstructor. eassumption.
           exact Hd2. reflexivity.
         }
@@ -652,12 +652,12 @@ Proof.
   * (* same as above *)
     apply H0 in H as H'. 2: lia.
     destruct H' as [res [k [ll [Hres [Hd Hlt]]]]].
-    eapply frame_indep_nil in Hd.
-    eapply term_step_term in H. 2: exact Hd. simpl in *.
+    eapply frame_indep_nil_labeled in Hd.
+    eapply term_step_term_labeled in H. 2: exact Hd. simpl in *.
     inv Hres.
     - do 3 eexists. split. 2: split.
       2: {
-        eapply transitive_eval. exact Hd.
+        eapply transitive_eval_labeled. exact Hd.
         eapply step_trans. constructor. reflexivity. apply step_refl.
         reflexivity.
       }
@@ -671,7 +671,7 @@ Proof.
       }
       do 3 eexists. split. 2: split.
       2: {
-        eapply transitive_eval. exact Hd.
+        eapply transitive_eval_labeled. exact Hd.
         eapply step_trans. constructor. exact Hd2.
         reflexivity.
       }
@@ -680,7 +680,7 @@ Proof.
 Qed.
 
 (* TODO: move this to Basics.v *)
-Corollary prefix_drop : forall {A} (l0 l1 : list A) ,
+Proposition prefix_drop : forall {A} (l0 l1 : list A) ,
             l0 `prefix_of` l1 -> 
             forall l2,
               l2 = drop (length l0) l1 ->
@@ -692,7 +692,7 @@ Proof.
     reflexivity.
 Qed.
 
-Corollary Private_params_exp_eval_empty :
+Lemma Private_params_exp_eval_empty :
   forall exps ident vl Fs (e : Exp) n l,
   | FParams ident vl exps :: Fs, e | l – n ↓ ->
   (forall m : nat,
@@ -708,13 +708,13 @@ Proof.
   induction exps; intros.
   * apply H0 in H as H'. 2: lia.
     destruct H' as [res [k [l' [Hres [Hd [Hlt Hpref]]]]]].
-    eapply frame_indep_nil in Hd as Hlia.
-    eapply frame_indep_nil in Hd.
-    eapply term_step_term in H as Hlia2. 2: exact Hlia. simpl in *.
+    eapply frame_indep_nil_labeled in Hd as Hlia.
+    eapply frame_indep_nil_labeled in Hd.
+    eapply term_step_term_labeled in H as Hlia2. 2: exact Hlia. simpl in *.
     inv Hres.
     - do 3 eexists. split. 2: split. 3: split.
       2: {
-        eapply transitive_eval. exact Hd.
+        eapply transitive_eval_labeled. exact Hd.
         eapply step_trans. constructor. reflexivity. apply step_refl.
         reflexivity.
       }
@@ -726,7 +726,7 @@ Proof.
       + auto.
       + do 3 eexists. split. 2: split. 3: split.
         2: {
-          eapply transitive_eval. exact Hd.
+          eapply transitive_eval_labeled. exact Hd.
           eapply step_trans. econstructor. eassumption. apply step_refl.
           reflexivity.
         }
@@ -740,12 +740,12 @@ Proof.
       (* if create_result was a function application: *)
       + inv H1. apply H0 in H8 as H8'. 2: lia.
         destruct H8' as [res2 [k2 [l2 [Hres2 [Hd2 [Hlt2 Hpref2]]]]]].
-        eapply frame_indep_nil in Hd2 as Hlia3.
-        eapply frame_indep_nil in Hd2.
-        eapply term_step_term in H8. 2: exact Hlia3.
+        eapply frame_indep_nil_labeled in Hd2 as Hlia3.
+        eapply frame_indep_nil_labeled in Hd2.
+        eapply term_step_term_labeled in H8. 2: exact Hlia3.
         do 3 eexists. split. 2: split. 3: split.
         2: {
-          eapply transitive_eval. exact Hd.
+          eapply transitive_eval_labeled. exact Hd.
           eapply step_trans. econstructor. eassumption.
           exact Hd2. reflexivity.
         }
@@ -762,13 +762,13 @@ Proof.
   * (* same as above *)
     apply H0 in H as H'. 2: lia.
     destruct H' as [res [k [l' [Hres [Hd Hlt]]]]].
-    eapply frame_indep_nil in Hd as Hlia.
-    eapply frame_indep_nil in Hd.
-    eapply term_step_term in H as Hlia2. 2: exact Hlia. simpl in *.
+    eapply frame_indep_nil_labeled in Hd as Hlia.
+    eapply frame_indep_nil_labeled in Hd.
+    eapply term_step_term_labeled in H as Hlia2. 2: exact Hlia. simpl in *.
     inv Hres.
     - do 3 eexists. split. 2: split. 3: split.
       2: {
-        eapply transitive_eval. exact Hd.
+        eapply transitive_eval_labeled. exact Hd.
         eapply step_trans. constructor. reflexivity. apply step_refl.
         reflexivity.
       }
@@ -786,7 +786,7 @@ Proof.
       }
       do 3 eexists. split. 2: split. 3: split.
       2: {
-        eapply transitive_eval. exact Hd.
+        eapply transitive_eval_labeled. exact Hd.
         eapply step_trans. constructor.
         exact Hd2.
         reflexivity.
@@ -802,7 +802,7 @@ Proof.
       by auto.
 Qed.
 
-Corollary Private_term_empty_case l:
+Lemma Private_term_empty_case l:
   forall Fs (vs : ValSeq) n (ls : SideEffectList),
   (forall (m : nat) ,
   m < n ->
@@ -825,14 +825,14 @@ Proof.
     - (* matching first pattern *)
       apply IH in H6 as HH. 2: lia. destruct HH as [i [li [Hdgr [Hlt Hprefi]]]].
       apply semantic_iff_termination in Hdgr as [gr [Hgr Hdgr]]. (* guard result *)
-      eapply frame_indep_nil in Hdgr as Hlia.
-      eapply frame_indep_nil in Hdgr.
-      eapply term_step_term in H6.
+      eapply frame_indep_nil_labeled in Hdgr as Hlia.
+      eapply frame_indep_nil_labeled in Hdgr.
+      eapply term_step_term_labeled in H6.
       2: exact Hlia. simpl in *. inv Hgr.
       + (* guard is an exception *) inv H6.
         exists (RExc (cl, v1, v2)), (1 + (i + 1)). eexists. split; auto. split.
         2: split. 2: lia.
-        econstructor. constructor. exact H5. eapply transitive_eval.
+        econstructor. constructor. exact H5. eapply transitive_eval_labeled.
         exact Hdgr. econstructor. constructor. congruence. constructor.
         1-2: reflexivity. rewrite <- app_nil_r. do 2 rewrite app_nil_r. assumption.
       + inv H6.
@@ -840,14 +840,14 @@ Proof.
            apply IH in H7 as HH. 2: lia.
            destruct HH as [j [lj [Hdcl [Hlt2 Hprefj]]]].
            apply semantic_iff_termination in Hdcl as [clr [Hclr Hdcl]]. (* clause result *)
-           eapply frame_indep_nil in Hdcl. simpl in *.
+           eapply frame_indep_nil_labeled in Hdcl. simpl in *.
            assert (⟨ [FCase2 vs e2.[list_subst vs' idsubst] l], RValSeq [VLit "true"%string] ⟩ -[1 , []]->ₗ
            ⟨ [], e2.[list_subst vs' idsubst] ⟩). {
              econstructor. constructor. constructor.
              reflexivity.
            }
-           epose proof (transitive_eval Hdgr H).
-           epose proof (transitive_eval H0 Hdcl).
+           epose proof (transitive_eval_labeled _ Hdgr _ H).
+           epose proof (transitive_eval_labeled _ H0 _ Hdcl).
            exists clr, (1 + (i + 1 + j)). eexists. split; auto.
            split. 2: split. 2: lia.
            econstructor. apply eval_step_case_match; eassumption.
@@ -860,7 +860,7 @@ Proof.
            }
            exists res, (1 + (i + S j)). eexists. split. 2: split. auto. 2: split. 2: lia.
            econstructor. apply eval_step_case_match. eassumption.
-           eapply transitive_eval. exact Hdgr.
+           eapply transitive_eval_labeled. exact Hdgr.
            econstructor. constructor. exact HD. reflexivity. reflexivity.
            destruct Hprefi. subst.
            apply prefix_app. rewrite drop_app_length in Hpref. assumption.
@@ -932,14 +932,14 @@ Proof.
     destruct_scopes. apply H in H3 as HD1; auto.
     destruct HD1 as [k1 [l1 [D1 [Hlia1 Hpref]]]].
     apply semantic_iff_termination in D1 as [res1 [Hres1 Hr1]].
-    eapply frame_indep_nil in Hr1 as Hr1'.
-    eapply frame_indep_nil in Hr1.
-    eapply term_step_term in H3.
+    eapply frame_indep_nil_labeled in Hr1 as Hr1'.
+    eapply frame_indep_nil_labeled in Hr1.
+    eapply term_step_term_labeled in H3.
     2: exact Hr1. simpl in *.
     inv Hres1.
     (* moduleexp Exception *)
     - inv H3. do 2 eexists. split. constructor.
-      eapply step_term_term_plus. exact Hr1'. constructor.
+      eapply step_term_term_plus_labeled. exact Hr1'. constructor.
       congruence. constructor. constructor; auto. split. lia.
       rewrite app_nil_r. assumption.
     (* moduleexp Value *)
@@ -947,15 +947,15 @@ Proof.
       apply H in H6 as HD2; auto. 2: lia.
       destruct HD2 as [k2 [l2 [D2 [Hlia2 Hpref2]]]].
       apply semantic_iff_termination in D2 as [res2 [Hres2 Hr2]].
-      eapply frame_indep_nil in Hr2 as Hr2'.
-      eapply frame_indep_nil in Hr2.
-      eapply term_step_term in H6.
+      eapply frame_indep_nil_labeled in Hr2 as Hr2'.
+      eapply frame_indep_nil_labeled in Hr2.
+      eapply term_step_term_labeled in H6.
       2: exact Hr2. simpl in *.
       inv Hres2.
       (* funexp exception *)
       + inv H6. do 2 eexists. split. constructor.
-        eapply step_term_term_plus. exact Hr1'. constructor.
-        eapply step_term_term_plus. exact Hr2'. constructor.
+        eapply step_term_term_plus_labeled. exact Hr1'. constructor.
+        eapply step_term_term_plus_labeled. exact Hr2'. constructor.
         congruence. constructor. constructor; auto. split. lia.
         rewrite app_nil_r. destruct Hpref2. symmetry in H0.
         epose proof (prefix_drop l1 l Hpref (l2 ++ x) H0).
@@ -965,8 +965,8 @@ Proof.
       + inv H6. destruct el. (* tricks to avoid RBox *)
         ** inv H5. do 2 eexists. split.
            constructor.
-           eapply step_term_term_plus. exact Hr1'. constructor.
-           eapply step_term_term_plus. exact Hr2'. constructor.
+           eapply step_term_term_plus_labeled. exact Hr1'. constructor.
+           eapply step_term_term_plus_labeled. exact Hr2'. constructor.
            epose proof (cool_params_0_l [] (ICall v f0) [] _ l0 []). simpl in H0.
            apply H0.
            congruence. exact H6.
@@ -1011,8 +1011,8 @@ Proof.
            destruct HD3 as [res3 [k3 [l3 [Hres3 [Hd3 [Hlt3 Hpref3]]]]]].
            do 2 eexists. split. 2: split.
            constructor.
-           eapply step_term_term_plus. exact Hr1'. constructor.
-           eapply step_term_term_plus. exact Hr2'. constructor.
+           eapply step_term_term_plus_labeled. exact Hr1'. constructor.
+           eapply step_term_term_plus_labeled. exact Hr2'. constructor.
            constructor. congruence.
            eapply semantic_iff_termination. eexists.
            split. 2: exact Hd3. auto. lia.
@@ -1055,13 +1055,13 @@ Proof.
      the number of case separations. *)
   * apply H in H3 as H3'. destruct H3' as [j [l1 [Hj [Hlt1 Hpref]]]]. 2: lia.
     apply semantic_iff_termination in Hj as [res [Hres Hr]].
-    eapply frame_indep_nil in Hr as Hlia1.
-    eapply frame_indep_nil in Hr. eapply term_step_term in H3.
+    eapply frame_indep_nil_labeled in Hr as Hlia1.
+    eapply frame_indep_nil_labeled in Hr. eapply term_step_term_labeled in H3.
     2: exact Hlia1. simpl in *.
     destruct l0. (* tricks to avoid RBox *)
     - inv Hres. (* exception result? *)
       + exists (2 + j). eexists. split. constructor.
-        eapply step_term_term. simpl. exact Hr. 2: lia.
+        eapply step_term_term_labeled. simpl. exact Hr. 2: lia.
         replace (S j - j) with 1 by lia.
         constructor. reflexivity. constructor. auto.
         inv H3. split. lia.
@@ -1071,7 +1071,7 @@ Proof.
         destruct (create_result_is_not_box (IApp v) [] res l0).
         ** assumption.
         ** exists (3 + j). eexists. split. constructor.
-           eapply step_term_term. exact Hr. 2: lia.
+           eapply step_term_term_labeled. exact Hr. 2: lia.
            replace (S (S j) - j) with 2 by lia.
            constructor. econstructor. congruence. eassumption.
            now constructor.
@@ -1087,7 +1087,7 @@ Proof.
         ** inv H0. apply H in H9 as H9'. 2: lia.
            destruct H9' as [i [l2 [Hd2 [Hlt2 Hpref2]]]].
            exists (1 + (j + 2 + i)). eexists. split. constructor.
-           eapply step_term_term. exact Hr. 2: lia.
+           eapply step_term_term_labeled. exact Hr. 2: lia.
            replace (j + 2 + i - j) with (2 + i) by lia.
            constructor. econstructor. congruence. eassumption. exact Hd2.
            split. lia. destruct Hpref. subst. rewrite drop_app_length in H3.
@@ -1100,7 +1100,7 @@ Proof.
            rewrite <- app_nil_r at 1. apply prefix_app. apply prefix_nil.
     - inv Hres.
       + exists (2 + j). eexists. split. constructor.
-        eapply step_term_term. exact Hr. 2: lia.
+        eapply step_term_term_labeled. exact Hr. 2: lia.
         replace (S j - j) with 1 by lia.
         constructor. reflexivity. constructor. auto.
         inv H3. split. lia. rewrite app_nil_r. assumption.
@@ -1117,8 +1117,8 @@ Proof.
         assert (⟨ [FApp1 (e :: l0)], RValSeq [v]⟩ -[2 , []]->ₗ ⟨ [FParams (IApp v) [] l0], e ⟩). {
           repeat econstructor. congruence.
         }
-        eapply (transitive_eval Hr) in H0.
-        eapply (transitive_eval H0) in Hd2.
+        eapply (transitive_eval_labeled _ Hr) in H0.
+        eapply (transitive_eval_labeled _ H0) in Hd2.
         do 2 eexists. split.
         constructor. apply semantic_iff_termination.
         eexists. split. 2: exact Hd2. assumption. split. lia.
@@ -1128,30 +1128,30 @@ Proof.
   * apply H in H3 as HH. 2: lia.
     destruct HH as [i [li [Hi [Hlt Hprefi]]]].
     apply semantic_iff_termination in Hi as [res [Hres Hr]].
-    eapply frame_indep_nil in Hr as Hlia1.
-    eapply frame_indep_nil in Hr.
-    eapply term_step_term in H3. 2: exact Hlia1.
+    eapply frame_indep_nil_labeled in Hr as Hlia1.
+    eapply frame_indep_nil_labeled in Hr.
+    eapply term_step_term_labeled in H3. 2: exact Hlia1.
     inv Hres. (* tail exception or not *)
     - exists (S i + 1). eexists.
       split. 2: split. 2: inv H3; lia.
       simpl. constructor. apply semantic_iff_termination.
-      exists (RExc (cl, v1, v2)). split; auto. eapply transitive_eval.
+      exists (RExc (cl, v1, v2)). split; auto. eapply transitive_eval_labeled.
       exact Hr. do 2 econstructor. reflexivity.
       rewrite app_nil_r. assumption.
     - inv H3. apply H in H5 as HH. 2: lia.
       destruct HH as [j [lj [Hj [Hltj Hprefj]]]].
       simpl in *. apply semantic_iff_termination in Hj as [hdres [Hr2 Hd2]].
-      eapply frame_indep_nil in Hd2 as Hlia2.
-      eapply frame_indep_nil in Hd2.
-      eapply term_step_term in H5. 2: exact Hlia2.
+      eapply frame_indep_nil_labeled in Hd2 as Hlia2.
+      eapply frame_indep_nil_labeled in Hd2.
+      eapply term_step_term_labeled in H5. 2: exact Hlia2.
       assert (⟨ [FCons1 hd], RValSeq [tl0] ⟩ -[1 , []]->ₗ ⟨[FCons2 tl0], hd⟩). {
         repeat econstructor.
       }
-      eapply (transitive_eval Hr) in H0.
-      eapply (transitive_eval H0) in Hd2.
+      eapply (transitive_eval_labeled _ Hr) in H0.
+      eapply (transitive_eval_labeled _ H0) in Hd2.
       inv Hr2. (* head exception or not *)
       + exists (1 + (i + (1 + (j + 1) ))). eexists. split.
-        simpl. constructor. eapply step_term_term.
+        simpl. constructor. eapply step_term_term_labeled.
         exact Hd2.
         replace (i + S (j + 1) - (i + 1 + j)) with 1 by lia.
         constructor. reflexivity. do 2 constructor; auto.
@@ -1162,7 +1162,7 @@ Proof.
         destruct Hprefj. rewrite drop_app_length in H2. rewrite H2.
         rewrite <- app_nil_r at 1. apply prefix_app. apply prefix_nil.
       + exists (1 + (i + (1 + (j + 1) ))). eexists. split.
-        simpl. constructor. eapply step_term_term.
+        simpl. constructor. eapply step_term_term_labeled.
         exact Hd2. inv H5.
         replace (i + S (j + 1) - (i + 1 + j)) with 1 by lia.
         destruct_foralls.
@@ -1173,29 +1173,29 @@ Proof.
   * apply H in H3 as HH. 2: lia.
     destruct HH as [i [li [Hi [Hlt Hprefi]]]].
     apply semantic_iff_termination in Hi as [res [Hres Hr]].
-    eapply frame_indep_nil in Hr as Hlia1.
-    eapply frame_indep_nil in Hr.
-    eapply term_step_term in H3. 2: exact Hlia1.
+    eapply frame_indep_nil_labeled in Hr as Hlia1.
+    eapply frame_indep_nil_labeled in Hr.
+    eapply term_step_term_labeled in H3. 2: exact Hlia1.
     inv Hres. (* tail exception or not *)
     - exists (S i + 1). eexists.
       split. 2: split. 2: inv H3; lia.
       simpl. constructor. apply semantic_iff_termination.
-      exists (RExc (cl, v1, v2)). split; auto. eapply transitive_eval.
+      exists (RExc (cl, v1, v2)). split; auto. eapply transitive_eval_labeled.
       exact Hr. do 2 econstructor. reflexivity.
       rewrite app_nil_r. assumption.
     - inv H3. apply H in H8 as HH. 2: lia.
       destruct HH as [j [lj [Hj [Hltj Hprefj]]]].
       simpl in *. apply semantic_iff_termination in Hj as [hdres [Hr2 Hd2]].
-      eapply frame_indep_nil in Hd2 as Hlia2.
-      eapply term_step_term in H8. 2: exact Hlia2.
+      eapply frame_indep_nil_labeled in Hd2 as Hlia2.
+      eapply term_step_term_labeled in H8. 2: exact Hlia2.
       assert (⟨ [FLet (Datatypes.length vs) e2], RValSeq vs ⟩ -[1, []]->ₗ 
       ⟨ [], e2.[list_subst vs idsubst] ⟩). {
         repeat econstructor.
       }
-      eapply (transitive_eval Hr) in H0.
-      eapply (transitive_eval H0) in Hd2.
+      eapply (transitive_eval_labeled _ Hr) in H0.
+      eapply (transitive_eval_labeled _ H0) in Hd2.
       exists (1 + (i + (1 + j))). eexists. split. 2: split. 2: inv Hr2; inv H0; lia.
-      constructor. eapply step_term_term. exact Hd2.
+      constructor. eapply step_term_term_labeled. exact Hd2.
       replace (i + (1 + j) - (i + 1 + j)) with 0 by lia.
       now constructor.
       lia.
@@ -1207,29 +1207,29 @@ Proof.
   * apply H in H3 as HH. 2: lia.
     destruct HH as [i [li [Hi [Hlt Hprefi]]]].
     apply semantic_iff_termination in Hi as [res [Hres Hr]].
-    eapply frame_indep_nil in Hr as Hlia1.
-    eapply frame_indep_nil in Hr.
-    eapply term_step_term in H3. 2: exact Hlia1.
+    eapply frame_indep_nil_labeled in Hr as Hlia1.
+    eapply frame_indep_nil_labeled in Hr.
+    eapply term_step_term_labeled in H3. 2: exact Hlia1.
     inv Hres. (* tail exception or not *)
     - exists (S i + 1). eexists.
       split. 2: split. 2: inv H3; lia.
       simpl. constructor. apply semantic_iff_termination.
-      exists (RExc (cl, v1, v2)). split; auto. eapply transitive_eval.
+      exists (RExc (cl, v1, v2)). split; auto. eapply transitive_eval_labeled.
       exact Hr. do 2 econstructor. reflexivity.
       rewrite app_nil_r. assumption.
     - inv H3. apply H in H5 as HH. 2: lia.
       destruct HH as [j [lj [Hj [Hltj Hprefj]]]].
       simpl in *. apply semantic_iff_termination in Hj as [hdres [Hr2 Hd2]].
-      eapply frame_indep_nil in Hd2 as Hlia2.
-      eapply term_step_term in H5. 2: exact Hlia2.
+      eapply frame_indep_nil_labeled in Hd2 as Hlia2.
+      eapply term_step_term_labeled in H5. 2: exact Hlia2.
       assert (⟨ [FSeq e2], RValSeq [v] ⟩ -[1 , []]->ₗ
       ⟨ [], e2 ⟩). {
         repeat econstructor.
       }
-      eapply (transitive_eval Hr) in H0.
-      eapply (transitive_eval H0) in Hd2.
+      eapply (transitive_eval_labeled _ Hr) in H0.
+      eapply (transitive_eval_labeled _ H0) in Hd2.
       exists (1 + (i + (1 + j))). eexists. split. 2: split. 2: inv Hr2; inv H0; lia.
-      constructor. eapply step_term_term. exact Hd2.
+      constructor. eapply step_term_term_labeled. exact Hd2.
       replace (i + (1 + j) - (i + 1 + j)) with 0 by lia.
       now constructor.
       lia.
@@ -1243,13 +1243,13 @@ Proof.
   (* for case: list_length_ind on H3 (or structural could also be enough) *)
   * apply H in H3 as HH. 2: lia. destruct HH as [k1 [l1 [Hd1 [Hlt1 Hpref1]]]].
     apply semantic_iff_termination in Hd1 as [r1 [Hr Hd]].
-    eapply frame_indep_nil in Hd as Hlia1.
-    eapply frame_indep_nil in Hd.
-    eapply term_step_term in H3. 2: exact Hlia1.
+    eapply frame_indep_nil_labeled in Hd as Hlia1.
+    eapply frame_indep_nil_labeled in Hd.
+    eapply term_step_term_labeled in H3. 2: exact Hlia1.
     simpl in *.
     inv Hr. (* exception? *)
     + exists (1 + k1 + 1). eexists. split. 2: split. 2: inv H3; lia.
-      simpl. constructor. eapply step_term_term. exact Hd.
+      simpl. constructor. eapply step_term_term_labeled. exact Hd.
       replace (k1 + 1 - k1) with 1 by lia.
       constructor. reflexivity. do 2 constructor; auto. lia.
       rewrite app_nil_r. assumption.
@@ -1258,7 +1258,7 @@ Proof.
       Unshelve. 2: {
         intros. eapply H. lia. eassumption.
       }
-      pose proof (transitive_eval Hd Hd2).
+      pose proof (transitive_eval_labeled _ Hd _ Hd2).
       exists (S (k1 + k2)). eexists. split. 2: split. 2: lia.
       constructor.
       apply semantic_iff_termination. exists res. split. 2: exact H0.
@@ -1269,15 +1269,15 @@ Proof.
   * apply H in H3 as HH. 2: lia.
     destruct HH as [i [li [Hd [Hlt Hpref]]]].
     apply semantic_iff_termination in Hd as [r [Hres Hd]].
-    eapply frame_indep_nil in Hd as Hlia.
-    eapply frame_indep_nil in Hd.
-    eapply term_step_term in H3. 2: exact Hlia.
+    eapply frame_indep_nil_labeled in Hd as Hlia.
+    eapply frame_indep_nil_labeled in Hd.
+    eapply term_step_term_labeled in H3. 2: exact Hlia.
     simpl in *.
     inv Hres. (* exception or not *)
     - inv H3. (* 2: { inv H7. } *)
       apply H in H10 as [j [l2 [Hd2 [Hlt2 Hpref2]]]]. 2: lia.
       exists (1 + (i + (1 + j))). eexists. split. 2: split. 2: lia.
-      constructor. eapply step_term_term. exact Hd. 2: lia.
+      constructor. eapply step_term_term_labeled. exact Hd. 2: lia.
       replace (i + (1 + j) - i) with (S j) by lia.
       2: { destruct Hpref. subst. rewrite drop_app_length in Hpref2.
            apply prefix_app. exact Hpref2.
@@ -1286,7 +1286,7 @@ Proof.
     - inv H3.
       apply H in H10 as [j [l2 [Hd2 [Hlt2 Hpref2]]]]. 2: lia.
       exists (1 + (i + (1 + j))). eexists. split. 2: split. 2: lia.
-      constructor. eapply step_term_term. exact Hd. 2: lia.
+      constructor. eapply step_term_term_labeled. exact Hd. 2: lia.
       replace (i + (1 + j) - i) with (S j) by lia.
       2: { destruct Hpref. subst. rewrite drop_app_length in Hpref2.
            apply prefix_app. exact Hpref2.
@@ -1299,7 +1299,7 @@ Qed.
 (* sufficient to prove it for Exp, since value sequences and
    exceptions terminate in 0/1 step by definition in the
    empty stack (and RBox does not terminate!). *)
-Corollary term_eval_empty : forall x Fs (e : Exp) (He : EXPCLOSED e) (ls : SideEffectList) ,
+Corollary term_eval_empty_labeled : forall x Fs (e : Exp) (ls : SideEffectList) ,
   | Fs, e | ls – x ↓ ->
   exists res k lss ,
     is_result res /\
@@ -1312,7 +1312,7 @@ Proof.
   do 3 eexists; eauto.
 Qed.
 
-Corollary term_eval : forall x Fs (e : Exp) (He : EXPCLOSED e) (ls : SideEffectList) ,
+Corollary term_eval_labeled : forall x Fs (e : Exp) (ls : SideEffectList) ,
   | Fs, e | ls – x ↓ ->
   exists v k lss,
     is_result v /\
@@ -1322,13 +1322,13 @@ Corollary term_eval : forall x Fs (e : Exp) (He : EXPCLOSED e) (ls : SideEffectL
     .
 Proof.
   intros.
-  apply term_eval_empty in H as [r [k [lss [Hr [Hd Hlt]]]]].
+  apply term_eval_empty_labeled in H as [r [k [lss [Hr [Hd Hlt]]]]].
   exists r, k, lss. intuition.
-  eapply frame_indep_nil in Hd. exact Hd. auto.
+  eapply frame_indep_nil_labeled in Hd. exact Hd.
 Qed.
 
-Corollary term_eval_both :
-  forall x Fs (e : Exp) (He : EXPCLOSED e) (l : SideEffectList) , 
+Corollary term_eval_both_labeled :
+  forall x Fs (e : Exp) (l : SideEffectList) , 
   | Fs, e | l – x ↓ ->
   exists v k ls, is_result v /\
   ⟨ [], e ⟩ -[k , ls]->ₗ ⟨ [], v ⟩ /\
@@ -1336,135 +1336,257 @@ Corollary term_eval_both :
   k <= x /\
   ls `prefix_of` l.
 Proof.
-  intros. apply term_eval_empty in H as [r [k [ls [Hr [Hd [Hlt Hpref]]]]]].
+  intros. apply term_eval_empty_labeled in H as [r [k [ls [Hr [Hd [Hlt Hpref]]]]]].
   exists r, k, ls. intuition.
-  eapply frame_indep_nil in Hd. exact Hd.
-  assumption.
+  eapply frame_indep_nil_labeled in Hd. exact Hd.
 Qed.
 
-From CoreErlang.FrameStack Require Export
-  LabeledTermination.
+Lemma to_Exp_eval_labeled :
+  forall (vals : list Val) (exp : Exp) (exps : list Exp) ident Fs,
+   (ident = IMap -> exists n, length exps + length vals = 1 + 2*n) -> (* invariant for maps *)
+   exists k, ⟨Fs, to_Exp ident (map VVal vals ++ exp :: exps)⟩ -[k, []]->ₗ ⟨ FParams ident vals exps :: Fs, exp ⟩.
+Proof.
+  (* these subproofs are the same almost for most lang. elements
+     except for the number of initialisation steps *)
+  intros. destruct ident.
+  * destruct vals; simpl.
+    - eexists. econstructor. constructor.
+      econstructor. constructor. congruence.
+      constructor.
+      all: reflexivity.
+    - eexists. econstructor. constructor.
+      econstructor. constructor. congruence.
+      econstructor. constructor.
+      apply params_eval_labeled.
+      all: reflexivity.
+  * destruct vals; simpl.
+    - eexists. econstructor. constructor.
+      econstructor. constructor. congruence.
+      constructor.
+      all: reflexivity.
+    - eexists. econstructor. constructor.
+      econstructor. constructor. congruence.
+      econstructor. constructor.
+      apply params_eval_labeled.
+      all: reflexivity.
+  (* maps require special attention *)
+  * destruct vals; simpl.
+    - destruct exps.
+      + specialize (H eq_refl) as [n H]. simpl in H. lia.
+      + specialize (H eq_refl) as [n H]. simpl in H.
+        eexists. econstructor. constructor.
+        rewrite deflatten_flatten with (n := n). 2: lia.
+        constructor.
+        all: reflexivity.
+    - destruct vals.
+      + simpl. specialize (H eq_refl) as [n H].
+        eexists. econstructor. constructor.
+        econstructor. constructor.
+        econstructor. constructor.
+        simpl in H.
+        rewrite deflatten_flatten with (n := n). 2: lia.
+        constructor.
+        all: reflexivity.
+      + simpl. specialize (H eq_refl) as [n H].
+        eexists. econstructor. constructor.
+        econstructor. constructor.
+        econstructor. constructor.
+        econstructor. constructor.
+        simpl in H.
+        rewrite deflatten_flatten with (n := n).
+        2: rewrite length_app, length_map; slia.
+        apply params_eval_labeled.
+        all: reflexivity.
+  (***)
+  * destruct vals; simpl.
+    - eexists. econstructor. constructor.
+      econstructor. constructor.
+      econstructor. constructor.
+      econstructor. constructor.
+      econstructor. constructor.
+      econstructor. constructor. congruence.
+      constructor.
+      all: reflexivity.
+    - eexists. econstructor. constructor.
+      econstructor. constructor.
+      econstructor. constructor.
+      econstructor. constructor.
+      econstructor. constructor.
+      econstructor. constructor. congruence.
+      econstructor. constructor.
+      apply params_eval_labeled.
+      all: reflexivity.
+  * destruct vals; simpl.
+    - eexists. econstructor. constructor.
+      econstructor. constructor. congruence.
+      constructor.
+      all: reflexivity.
+    - eexists. econstructor. constructor.
+      econstructor. constructor. congruence.
+      econstructor. constructor.
+      apply params_eval_labeled.
+      all: reflexivity.
+  * destruct vals; simpl.
+    - eexists. econstructor. constructor.
+      econstructor. constructor.
+      econstructor. constructor.
+      econstructor. constructor. congruence.
+      constructor.
+      all: reflexivity.
+    - eexists. econstructor. constructor.
+      econstructor. constructor.
+      econstructor. constructor.
+      econstructor. constructor. congruence.
+      econstructor. constructor.
+      apply params_eval_labeled.
+      all: reflexivity.
+Qed.
+
+Corollary params_eval_VValues_labeled :
+ forall (vals : list Val) (Fs : list Frame),
+ ⟨ Fs, °EValues (map VVal vals)⟩ -[
+   2 + 2 * base.length vals, [] ]->ₗ ⟨ Fs, RValSeq vals ⟩.
+Proof.
+  intros. destruct vals.
+  * simpl. econstructor. constructor.
+    econstructor. econstructor. congruence. reflexivity.
+    constructor. all: reflexivity.
+  * simpl. econstructor. constructor.
+    econstructor. constructor. congruence.
+    econstructor. constructor.
+    pose proof params_eval_create vals IValues [] Fs v (RValSeq (v::vals)) None eq_refl.
+    replace (length vals + S (length vals + 0)) with
+            (1 + 2 * length vals) by lia.
+    simpl in *.
+    eassumption.
+    all: reflexivity.
+Qed.
 
 
-Corollary put_back : forall F e Fs (P : EXPCLOSED e) (P2 : FCLOSED F) (l : SideEffectList),
-  | F :: Fs, e |ₗ l ↓ -> | Fs, plug_f F e |ₗ l ↓.
+Theorem put_back_labeled :
+  forall F Fs (e : Exp) r k l,
+    FrameWf F -> (* required by map frames *)
+    is_result r -> (* required by special case frames *)
+    ⟨F :: Fs, e⟩ -[k, l]->ₗ ⟨[], r⟩
+  ->
+    exists j, ⟨Fs, plug_f F e⟩ -[j, l]->ₗ ⟨[], r⟩.
 Proof.
   destruct F; intros; simpl.
-  all: try now (inv H; exists (S x); constructor; auto).
-  * inv H. exists (3 + x). do 2 constructor. now inv P2.
-    now constructor.
-  * inv H. destruct ident; simpl; destruct_scopes.
-  (* These build on the same idea, however, calls, applications and maps are a bit different: *)
-  1-2, 5: destruct vl; destruct_foralls; simpl; [
-    eexists; do 2 constructor; [congruence | eassumption]
-    |
-    exists (4 + ((2 * length vl) + x)); do 2 constructor;
-    try congruence; constructor; auto;
-    eapply step_term_term with (l1 := []);
-    [
-      apply params_eval
-      |
-      simpl app;
-      now replace (S (2 * Datatypes.length vl + x) - (1 + 2 * Datatypes.length vl)) with x by lia
-      |
-      lia
-    ]
-  ]; auto.
-    - destruct_scopes. specialize (H6 eq_refl).
-      inv H6. destruct vl.
-      + simpl. destruct el.
-        ** simpl in H. congruence.
-        ** eexists. constructor.
-           erewrite deflatten_flatten. eassumption.
-           simpl in H. instantiate (1 := x0). lia.
-      + simpl. destruct vl; simpl.
-        ** eexists. do 2 constructor. now inv H4. constructor. simpl.
-           erewrite deflatten_flatten. eassumption.
-           simpl in H. instantiate (1 := x0). lia.
-        ** exists (5 + ((2 * length vl) + x)). do 2 constructor.
-           now inv H4. do 2 constructor. now destruct_foralls.
-           erewrite deflatten_flatten.
-           2: { rewrite length_app, length_map. simpl in *.
-                instantiate (1 := x0). lia. }
-           eapply step_term_term with (l1 := []).
-           apply params_eval. now destruct_foralls. simpl app. 2: lia.
-           now replace (S (2 * Datatypes.length vl + x) - (1 + 2 * Datatypes.length vl)) with x by lia.
-    - destruct vl; simpl.
-      + eexists. do 2 constructor. now inv H3. do 2 constructor. now inv H3.
-        do 2 constructor. congruence. eassumption.
-      + exists (8 + ((2 * length vl) + x)). do 2 constructor.
-        now inv H3. do 2 constructor. now inv H3.
-        do 2 constructor. congruence.
-        constructor. now inv H4.
-        eapply step_term_term with (l1 := []).
-        apply params_eval. now inv H4. simpl app. 2: lia.
-        now replace (S (2 * Datatypes.length vl + x) - (1 + 2 * Datatypes.length vl)) with x by lia.
-    - destruct vl; simpl.
-      + eexists. do 2 constructor. now inv H3. do 2 constructor. congruence. eassumption.
-      + exists (6 + ((2 * length vl) + x)). do 2 constructor.
-        now inv H3. do 2 constructor. congruence.
-        constructor. now inv H4.
-        eapply step_term_term with (l1 := []).
-        apply params_eval. now inv H4. simpl app. 2: lia.
-        now replace (S (2 * Datatypes.length vl + x) - (1 + 2 * Datatypes.length vl)) with x by lia.
-  * destruct H as [k D]. eexists. do 2 constructor. now inv P2. constructor.
-    eassumption.
-  * inv H. apply term_eval_both in H0 as H'. destruct H' as [res [k [ls [Hres [D0 [D1 [Hlt Hpref]]]]]]]. 2: assumption.
-    eapply term_step_term in H0. 2: eassumption.
-    clear D1. inv Hres.
-    - inv H0.
-      eexists. do 2 econstructor. eapply cool_params_0_l with (ls:=l) (l:=None).
-      congruence. reflexivity.
-      econstructor. reflexivity. cbn. eapply frame_indep_nil in D0.
-      do 2 rewrite idsubst_is_id_exp.
-      replace l with (ls ++ (drop (base.length ls) l)).
-      2: { destruct Hpref. rewrite e0. rewrite drop_app_length. reflexivity. }
-      eapply step_term_term_plus. eassumption. constructor. reflexivity.
+  all: try by (eexists; econstructor; [ constructor | eassumption | reflexivity]).
+  * eexists. econstructor. constructor.
+    econstructor. constructor.
+    econstructor. constructor. eassumption.
+    all: reflexivity.
+  (* parameter list frames: *)
+  * pose proof (to_Exp_eval_labeled vl e el ident Fs H) as [k0 X].
+    eexists.
+    eapply transitive_eval_labeled with (l := []). exact X.
+    exact H1.
+  (***)
+  * eexists.
+    econstructor. constructor.
+    econstructor. constructor.
+    econstructor. constructor. eassumption.
+    all: reflexivity.
+  (* Special "case" frame: *)
+  * (* independent evaluation of e *)
+    assert (terminates_in_k_sem_labeled (FCase2 lv ex le :: Fs) e k l) as X. {
+      exists r. split; eassumption.
+    }
+    apply semantic_iff_termination in X.
+    apply term_empty in X as [k0 [newl [X [Hk0 Hpref]]]].
+    eapply term_eval_empty_labeled in X as [res [i [newl2 [Hres [X [Hi Hpref2]]]]]].
+    eapply frame_indep_nil_labeled in X as X'.
+    replace k with (i+(k-i)) in H1 by lia.
+    pose proof (prefix_drop _ _ Hpref2 _ eq_refl) as HX.
+    pose proof (prefix_drop _ _ Hpref _ eq_refl) as HX2.
+    rewrite HX2, HX in H1. rewrite <- app_assoc in H1.
+    epose proof (transitive_eval_rev_labeled _ _ _ _ _ _ X' _ _ _ _ H1) as XX.
+    inv XX. clear X'.
+    inv Hres; inv H3.
+    (* exception result and vseq (true and false guard) result
+       can have different number of steps *)
+    (* exception *)
+    - eexists.
+      econstructor. constructor.
+      econstructor. constructor.
+      econstructor. econstructor. congruence. reflexivity.
+      econstructor. constructor. reflexivity.
+      simpl. do 2 rewrite idsubst_is_id_exp.
+      eapply frame_indep_nil_labeled in X as X'. eapply transitive_eval_labeled.
+      exact X'. clear X'. econstructor. constructor. reflexivity.
+      eapply frame_indep_nil_labeled in X.
+      replace k with (i+(k-i)) in H1 by lia.
+      epose proof (transitive_eval_rev_labeled _ _ _ _ _ _ X _ _ _ _ H1) as XX.
+      inv XX. inv H5. assert (k2 = k1) by lia. subst. exact H6.
+      all: try reflexivity.
+      simpl.
+      by rewrite <-HX, app_assoc, <-HX.
+    (* true guard *)
+    - eexists.
+      econstructor. constructor.
+      econstructor. constructor.
+      econstructor. econstructor. congruence. reflexivity.
+      econstructor. constructor. reflexivity.
+      simpl. do 2 rewrite idsubst_is_id_exp.
+      eapply frame_indep_nil_labeled in X. eapply transitive_eval_labeled.
+      exact X. clear X. econstructor. constructor.
       eassumption.
-    - inv H0.
-      + eexists. do 2 econstructor. eapply cool_params_0_l with (ls:=l) (l:=None).
-        congruence. reflexivity.
-        econstructor. reflexivity. do 2 rewrite idsubst_is_id_exp.
-        replace l with (ls ++ (drop (base.length ls) l)).
-        2: { destruct Hpref. rewrite H0. rewrite drop_app_length. reflexivity. }
-        eapply frame_indep_nil in D0. eapply step_term_term_plus.
-        eassumption. econstructor. eassumption.
-      + eexists (4 + (k + (7 + 2 * length lv + k0))). do 2 econstructor.
-        eapply cool_params_0_l with (ls:=l) (l:=None).
-        congruence. reflexivity.
-        econstructor. reflexivity. do 2 rewrite idsubst_is_id_exp.
-        replace l with (ls ++ (drop (base.length ls) l)).
-        2: { destruct Hpref. rewrite H0. rewrite drop_app_length. reflexivity. }
-        eapply frame_indep_nil in D0. eapply step_term_term_plus.
-        eassumption. constructor. econstructor.
-        reflexivity. cbn. do 2 constructor.
-        replace (map
-       (fun '(p, x0, y) =>
-        (p, x0.[upn (PatListScope p) idsubst],
-         y.[upn (PatListScope p) idsubst])) le) with le.
-        replace (map (fun x0 : Exp => x0.[idsubst]) (map VVal lv)) with (map VVal lv).
-        2: {
-          clear. induction lv; auto. simpl. rewrite idsubst_is_id_val.
-          now rewrite IHlv at 1.
-        }
-        2: {
-          clear. induction le; auto. simpl. destruct a, p.
-          rewrite idsubst_upn, <-IHle.
-          now do 2 rewrite idsubst_is_id_exp.
-        }
-        clear D0. do 2 econstructor.
-        destruct lv.
-        ** eapply cool_params_0_l with (l:=None).
-           congruence. reflexivity. simpl. eassumption.
-        ** simpl. destruct Hpref. rewrite H0. rewrite drop_app_length.
-           constructor. congruence. subst. rewrite drop_app_length in H7.
-           econstructor.
-           inv P2. now inv H3.
-           replace (length lv + S (length lv + 0)) with (1 + 2 * length lv).
-           replace x0 with ([] ++ x0).
-           eapply step_term_term_plus.
-           eapply params_eval_create with (eff':=None). inv P2. now inv H3. reflexivity.
-           cbn. eassumption. reflexivity. lia.
+      all: try reflexivity.
+      simpl.
+      by rewrite <-HX, app_assoc, <-HX.
+    (* false guard *)
+    - eexists.
+      econstructor. constructor.
+      econstructor. constructor.
+      econstructor. econstructor. congruence. reflexivity.
+      econstructor. constructor. reflexivity.
+      simpl. do 2 rewrite idsubst_is_id_exp.
+      eapply frame_indep_nil_labeled in X. eapply transitive_eval_labeled.
+      exact X. clear X. econstructor. constructor.
+      econstructor. constructor. reflexivity. cbn.
+      rewrite map_ext with (g := id). 2: {
+        intros. by rewrite idsubst_is_id_exp.
+      }
+      rewrite map_id.
+      rewrite map_ext with (g := id). 2: {
+        intros. destruct a as [[pl g] b].
+        rewrite idsubst_upn.
+        by do 2 rewrite idsubst_is_id_exp.
+      }
+      rewrite map_id.
+      econstructor. constructor.
+      econstructor. constructor.
+      econstructor. constructor.
+      eapply transitive_eval_labeled.
+      apply params_eval_VValues_labeled. eassumption.
+      all: try reflexivity. simpl.
+      by rewrite <-HX, app_assoc, <-HX.
+Qed.
+
+Corollary put_back_term : forall F (e : Exp) Fs l, FrameWf F ->
+  | F :: Fs, e |ₗ l ↓ -> | Fs, plug_f F e |ₗ l ↓.
+Proof.
+  intros.
+  destruct H0. apply semantic_iff_termination in H0.
+  destruct H0 as [res [Hres H0]].
+  apply put_back_labeled in H0; try assumption.
+  destruct H0. exists x0.
+  apply semantic_iff_termination. eexists. split; eassumption.
+Qed.
+
+Corollary transitive_eval_rev_lt_labeled :
+  forall {Fs r Fs' r' k1} l1, ⟨Fs, r⟩ -[k1, l1]->ₗ ⟨Fs', r'⟩ ->
+    forall {Fs'' r'' k2} l2, k2 <= k1 -> l2 `prefix_of` l1
+      -> ⟨Fs, r⟩ -[k2, l2]->ₗ ⟨Fs'', r''⟩ ->
+      ⟨Fs'', r''⟩ -[k1 - k2, drop (length l2) l1]->ₗ ⟨Fs', r'⟩.
+Proof.
+  intros.
+  replace k1 with (k2 + (k1 - k2)) in H by lia.
+  replace l1 with (l2 ++ drop (length l2) l1) in H. 2: {
+    eapply prefix_drop in H1. 2: reflexivity. by rewrite H1 at 2.
+  }
+  eapply transitive_eval_rev_labeled in H. 2: eassumption. assumption.
 Qed.
 
 Ltac inv_term_labeled :=
@@ -1472,101 +1594,127 @@ Ltac inv_term_labeled :=
   | [H : | _, _ | _ – _ ↓ |- _] => inv H
   end.
 
-Corollary put_back_rev : forall F e Fs (P : EXPCLOSED e) (l : SideEffectList) , FCLOSED F ->
+Lemma transitive_contradiction_labeled :
+  forall k1 fs r fs' r' k2 l1 l2 r'', is_result r'' ->
+    ⟨fs, r⟩ -[k1, l1]->ₗ ⟨fs', r'⟩ ->
+    ⟨fs, r⟩ -[k2, l2]->ₗ ⟨[], r''⟩ ->
+    k2 < k1 ->
+    False.
+Proof.
+  induction k1; intros.
+  * lia.
+  * inv H0. inv H1.
+    - by apply value_nostep_labeled in H4.
+    - eapply IHk1.
+      + eassumption.
+      + eassumption.
+      + eapply step_determinism_labeled in H0. 2: exact H4.
+        destruct_and!. subst. eassumption.
+      + lia.
+Qed.
+
+Theorem put_back_rev_labeled :
+  forall F Fs (e : Exp) r k l,
+    FrameWf F -> (* required by map frames *)
+    is_result r -> (* required by special case frames *)
+    ⟨Fs, plug_f F e⟩ -[k, l]->ₗ ⟨[], r⟩
+  ->
+    exists j, ⟨F :: Fs, e⟩ -[j, l]->ₗ ⟨[], r⟩.
+Proof.
+  destruct F; intros; simpl in *.
+  all: try by (inv H1; try inv_result; inv H2;
+    eexists; eassumption).
+  * inv H1; try inv_result. inv H2.
+    inv H3. inv H1.
+    inv H2. inv H1.
+    eexists; eassumption.
+  (* parameter list frame: *)
+  * pose proof (to_Exp_eval_labeled vl e el ident Fs H) as [k0 X].
+    assert (k0 <= k \/ k0 > k) as [Hlt | Hlt] by lia.
+    - opose proof (transitive_eval_rev_lt_labeled _ H1 _ Hlt _ X).
+      apply prefix_nil.
+      eexists. eassumption.
+    (* k0 > k cannot happen: *)
+    - by eapply transitive_contradiction_labeled in H1.
+  * inv H1; try inv_result. inv H2.
+    inv H3. inv H1.
+    inv H2. inv H1.
+    eexists; eassumption.
+  (* special "case" frame *)
+  * inv H1. inv_result. inv H2.
+    inv H3. inv H1.
+    inv H2. inv H1. simpl in H10. invSome.
+    inv H3. inv H1. simpl in *. invSome.
+    simpl in *.
+    do 2 rewrite idsubst_is_id_exp in H2.
+    (* extract independent evaluation of e: *)
+    assert (terminates_in_k_sem_labeled (FCase2 [] ex
+      [([], ˝ VLit "true"%string,
+        ° ECase (° EValues (map VVal lv)) le)] :: Fs) e k l) as X. {
+      exists r. split; eassumption.
+    }
+    apply semantic_iff_termination in X.
+    eapply term_eval_empty_labeled in X as [res [i [newl [Hres [X [Hi Hpref]]]]]].
+    (***)
+    eapply frame_indep_nil_labeled in X as X'.
+    pose proof (transitive_eval_rev_lt_labeled _ H2 _ Hi Hpref X') as XX.
+    clear X' H2.
+    (* check what's the guard result: exception, false, or true *)
+    inv XX. inv Hres; inv H2.
+    (* exception *)
+    - eexists.
+      eapply frame_indep_nil_labeled in X.
+      pose proof (prefix_drop _ _ Hpref _ eq_refl). rewrite H2.
+      eapply transitive_eval_labeled.
+      exact X. econstructor. constructor. reflexivity.
+      eassumption.
+      reflexivity.
+    (* true - proof is the same as in the previous case *)
+    - eexists.
+      eapply frame_indep_nil_labeled in X.
+      pose proof (prefix_drop _ _ Hpref _ eq_refl). rewrite H2.
+      eapply transitive_eval_labeled.
+      exact X. econstructor. constructor.
+      eassumption.
+      reflexivity.
+    (* false *)
+    - inv H3. inv H2.
+      simpl in H15. invSome. simpl in *.
+      rewrite map_ext with (g := id) in H4. 2: {
+        intros. by rewrite idsubst_is_id_exp.
+      }
+      rewrite map_id in H4.
+      rewrite map_ext with (g := id) in H4. 2: {
+        intros. destruct a as [[pl g] b].
+        rewrite idsubst_upn.
+        by do 2 rewrite idsubst_is_id_exp.
+      }
+      rewrite map_id in H4. inv H4. inv H2.
+      inv H3. inv H2.
+      inv H4. inv_result. inv H2.
+      pose proof (params_eval_VValues_labeled lv (FCase1 le :: fs')).
+      assert (k0 >= 2 + 2 * base.length lv \/ k0 < 2 + 2 * base.length lv) as [Hlt | Hlt] by lia.
+      + opose proof (transitive_eval_rev_lt_labeled _ H3 _ Hlt _ H2) as XX.
+        apply prefix_nil.
+        eexists.
+        eapply frame_indep_nil_labeled in X.
+        pose proof (prefix_drop _ _ Hpref _ eq_refl). rewrite H4.
+        eapply transitive_eval_labeled. exact X.
+        econstructor. constructor.
+        exact XX.
+        simpl. by rewrite drop_0.
+      (* k0 should be greater; therefore, this is a contradiction *)
+      + by eapply transitive_contradiction_labeled in H2.
+Qed.
+
+
+Theorem put_back_rev_term_labeled : forall F e Fs l, FrameWf F ->
   | Fs, plug_f F e |ₗ l ↓ -> | F :: Fs, e |ₗ l ↓.
 Proof.
-  destruct F; intros; simpl.
-  all: try now (inv H0; cbn in *; inv_term_labeled; [eexists;eassumption | inv H0]).
-  * inv H0. cbn in *. inv H1.
-    - inv H6. inv H3. eexists. exact H7.
-    - inv H0.
-  * cbn. inv H0. destruct ident; simpl in H1.
-    1-2, 5: inv_term_labeled; [
-        destruct vl; inv_term_labeled;
-         [eexists; eassumption
-         |inv H9; eapply term_step_term in H3;[|apply params_eval]]; inv H; destruct_foralls; auto;
-         eexists; eassumption
-        |inv H0
-      ].
-    (* again, map, call and apply need special care: *)
-    - destruct_scopes. specialize (H7 eq_refl). inv H7. destruct vl.
-      + destruct el.
-        ** simpl in H. congruence.
-        ** inv H1. 2: inv H0. erewrite deflatten_flatten in H10.
-           2: { instantiate (1 := x0). simpl in H. lia. }
-           eexists. eassumption.
-      + destruct vl; simpl in *.
-        ** inv H1. 2: inv H0. erewrite deflatten_flatten in H10.
-           2: { instantiate (1 := x0). simpl in H. lia. }
-           do 2 inv_term_labeled. eexists. eassumption.
-        ** inv_term_labeled. 2: inv H0. erewrite deflatten_flatten in H10.
-           2: { instantiate (1 := x0). simpl in H.
-             rewrite length_app, length_map. slia. }
-           do 3 inv_term_labeled.
-           eapply term_step_term in H7;[|apply params_eval].
-           eexists; eassumption.
-           now destruct_foralls.
-    - inv_term_labeled. 2: inv H0. do 3 inv_term_labeled. destruct vl; inv_term_labeled.
-      + inv_term_labeled. eexists. eassumption.
-      + do 2 inv_term_labeled. eapply term_step_term in H5;[|apply params_eval].
-        eexists. eassumption.
-        inv H. now destruct_foralls.
-    - inv_term_labeled. 2: inv H0. inv_term_labeled. destruct vl; inv_term_labeled.
-      + inv_term_labeled. eexists. eassumption.
-      + do 2 inv_term_labeled. eapply term_step_term in H4;[|apply params_eval].
-        eexists. eassumption.
-        inv H. now destruct_foralls.
-  * simpl in *. inv H. destruct H0 as [k D]. inv_term_labeled. 2: { inv H. }
-    do 2 inv_term_labeled. eexists. exact H9.
-  * inv H0. cbn in *. inv H1. 2: inv H0. inv H6. inv H2. cbn in H8.
-    inv H8; cbn in *; try invSome; invSome. simpl in H12; do 2 rewrite idsubst_is_id_exp in H12.
-    rename H12 into H5.
-    apply term_eval_both in H5 as T. simpl.
-    destruct T as [res [l [sl [Hres [D0 [D1 [Hlia Hpref]]]]]]].
-    eapply term_step_term in H5. 2: eassumption. 2: auto.
-    clear D1. inv Hres.
-    - inv H5. eapply frame_indep_nil in D0.
-      simpl. destruct Hpref. subst. eexists. eapply step_term_term_plus.
-      eassumption. constructor. reflexivity. rewrite drop_app_length in H10. eassumption.
-    - inv H5.
-      + eapply frame_indep_nil in D0.
-        destruct Hpref. subst. rewrite drop_app_length in H9.
-        eexists.
-        eapply step_term_term_plus. eassumption.
-        cbn in *. clear D0. eapply step_case_true_l. eassumption.
-      + destruct Hpref. subst. rewrite drop_app_length in H9.
-        inv H9; inv H13. simpl in H5. inv H5. inv H11. inv H8. 2: inv_val.
-        replace (map
-       (fun '(p, x0, y) =>
-        (p, x0.[upn (PatListScope p) (list_subst vs' idsubst)],
-         y.[upn (PatListScope p) (list_subst vs' idsubst)])) le) with le in H5.
-        replace (map (fun x0 : Exp => x0.[(list_subst vs' idsubst)]) (map VVal lv)) with (map VVal lv) in H5.
-        2: {
-          inv H12. clear.
-          induction lv; auto. simpl in *.
-          rewrite idsubst_is_id_val.
-          rewrite <- IHlv. reflexivity.
-        }
-        2: {
-          inv H12. clear.
-          induction le; auto. rewrite map_cons.
-          rewrite <-IHle. simpl. do 2 induction a. rewrite idsubst_upn.
-          do 2 rewrite idsubst_is_id_exp. reflexivity.
-        }
-        inv H12. destruct lv.
-        ** inv H5. cbn in H8. invSome.
-           eapply frame_indep_nil in D0.
-           simpl in H7.
-           eexists.
-           eapply step_term_term_plus. eassumption.
-           eapply step_case_false_l. eassumption.
-        ** inv H5. inv H13. eapply term_step_term in H6.
-           2: eapply params_eval_create. 2: { inv H. now inv H8. }
-           2: { reflexivity. }
-           simpl in H6.
-           eapply frame_indep_nil in D0. eexists.
-           eapply step_term_term_plus. eassumption.
-           eapply step_case_false_l. eassumption.
-(*   * simpl in H0. repeat deriv. (* receive is not evaluated at this level *)
-  * simpl in H0. repeat deriv. (* receive is not evaluated at this level *) *)
+  intros.
+  destruct H0. apply semantic_iff_termination in H0.
+  destruct H0 as [res [Hres H0]].
+  apply put_back_rev_labeled in H0; try assumption.
+  destruct H0. exists x0.
+  apply semantic_iff_termination. eexists. split; eassumption.
 Qed.
